Add BatchedGEMM

src/lib/data/Kuiper.Array3.fst
@@ -1,4 +1,5 @@
 module Kuiper.Array3
+friend Kuiper.Array2 // Should remove
 #lang-pulse
 
 open Kuiper
@@ -238,4 +239,97 @@ fn implode
   forevery_ext _ (fun (i : abs (desc d0 d1 d2)) -> Cell a i |-> Frac f (acc (tr_val s) i));
   T.tensor_implode a;
   fold pts_to a #f s;
+}
+
+inline_for_extraction noextract
+let page
+  (#et : Type0)
+  (#d0 #d1 #d2 : erased nat)
+  (#l : layout d0 d1 d2)
+  (a : t et l)
+  (i : erased nat{i < d0})
+  : Array2.t et (page_layout a i)
+  = Array2.from_array (page_layout a i) (T.core (T.sliceof a 0 i))
+
+let page_is_global
+  (#et : Type0) (#d0 #d1 #d2 : nat) (#l : layout d0 d1 d2)
+  (a : t et l) (i : erased nat{i < d0})
+  : Lemma (ensures Array2.is_global (page a i) <==> is_global a)
+          [SMTPat (page a i)]
+  = admit() // Fix
+
+ghost
+fn extract_page
+  (#et : Type0)
+  (#d0 #d1 #d2 : nat)
+  (#l : layout d0 d1 d2)
+  (a : t et l)
+  (i : natlt d0)
+  (#f : perm) (#s : EMatrix3.t et d0 d1 d2)
+  requires
+    a |-> Frac f s
+  ensures
+    page a i |-> Frac f (EMatrix3.slice_page s i) **
+    (forall* (s' : EMatrix.ematrix et d1 d2).
+      page a i |-> Frac f s' @==>
+      a |-> Frac f (EMatrix3.upd_page s i s'))
+{
+  unfold pts_to a #f s;
+  T.tensor_extract_slice a 0 i #f #(tr_val s);
+
+  assert pure (Chest.equal
+    (chest_slice 0 i (tr_val s))
+    (Array2.tr_val (EMatrix3.slice_page s i)));
+  rewrite T.sliceof a 0 i |-> Frac f (chest_slice 0 i (tr_val s))
+       as page a i |-> Frac f (EMatrix3.slice_page s i);
+
+  intro_forall
+    #_
+    #(fun (s' : EMatrix.ematrix et d1 d2) ->
+      page a i |-> Frac f s'
+      @==> a |-> Frac f (EMatrix3.upd_page s i s'))
+    (forall* (s' : chest (modulo_i 0 (desc d0 d1 d2)) et).
+      sliceof a 0 i |-> Frac f s'
+      @==> a |-> Frac f (chest_update_slice 0 i (tr_val s) s'))
+    fn s' {
+      intro_trade
+        (page a i |-> Frac f s')
+        (a |-> Frac f (EMatrix3.upd_page s i s'))
+        (forall* (s' : chest (modulo_i 0 (desc d0 d1 d2)) et).
+              sliceof a 0 i |-> Frac f s'
+              @==> a |-> Frac f (chest_update_slice 0 i (tr_val s) s'))
+        fn _ {
+          assert pure (modulo_i 0 (desc d0 d1 d2) == Array2.desc d1 d2);
+          let w : chest (modulo_i 0 (desc d0 d1 d2)) et = Array2.tr_val s';
+          elim_forall w;
+          rewrite Array2.pts_to (page a i) #f s'
+               as sliceof a 0 i |-> Frac f w;
+          elim_trade _ _;
+          rewrite each chest_update_slice 0 i (tr_val s) w
+               as tr_val (EMatrix3.upd_page s i s');
+          fold pts_to a #f (EMatrix3.upd_page s i s');
+          ();
+        };
+    };
+  ();
+}
+
+ghost
+fn extract_page_ro
+  (#et : Type0)
+  (#d0 #d1 #d2 : nat)
+  (#l : layout d0 d1 d2)
+  (a : t et l)
+  (i : natlt d0)
+  (#f : perm) (#s : EMatrix3.t et d0 d1 d2)
+  requires
+    a |-> Frac f s
+  ensures
+    factored
+      (page a i |-> Frac f (EMatrix3.slice_page s i))
+      (a |-> Frac f s)
+{
+  extract_page a i;
+  elim_forall (EMatrix3.slice_page s i);
+  assert pure (EMatrix3.equal (EMatrix3.upd_page s i (EMatrix3.slice_page s i)) s);
 }
