src/klas/Klas.GEMM.Batched.fst
@@ -1,0 +1,7 @@
+module Klas.GEMM.Batched
+
+#lang-pulse
+open Kuiper
+module K = Kuiper.Kernel.BatchedGEMM
+
+let batched_gemm_f32 = K.batched_gemm_f32
